cava/monad-examples/UnsignedAdderExamples.v
@@ -51,36 +51,43 @@ Definition bv5_30 := N2Bv_sized 5 30.
 (* Test adders with no bit-growth and equal-sized inputs                      *)
 (******************************************************************************)
 
-Definition addNSim {sz: nat} (a: Bvector sz) (b: Bvector sz) :
-                   ident (Bvector sz)
+Definition addN {m bit} `{Cava m bit} {sz: nat}
+                (a: Vector.t bit sz) (b: Vector.t bit sz) :
+                m (Vector.t bit sz)
   := addNN a b.
   
 (* Check 0 + 0 = 0 *)
-Example add0_0 : combinational (addNSim bv4_0 bv4_0) = bv4_0.
+Example add0_0 : combinational (addN bv4_0 bv4_0) = bv4_0.
+Proof. reflexivity. Qed.
+
+(* Check 15 + 1 = 0 *)
+Example add15_1 : combinational (addN bv4_15 bv4_1) = bv4_0.
 Proof. reflexivity. Qed.
 
 (******************************************************************************)
 (* Unsigned addition with growth examples.                                                *)
 (******************************************************************************)
 
-Definition addSim {aSize bSize: nat} (a: Bvector aSize) (b: Bvector bSize) :
-                   ident (Bvector (1 + max aSize bSize))
-  := unsignedAdd a b.
+Definition adderGrowth {m bit} `{Cava m bit} {aSize bSize: nat}
+                       (ab: Vector.t bit aSize * Vector.t bit bSize) :
+                       m (Vector.t bit (1 + max aSize bSize)) :=
+  let (a, b) := ab in                     
+  unsignedAdd a b.
 
 (* Check 0 + 0 = 0 *)
-Example add5_0_0 : combinational (addSim bv4_0 bv4_0) = bv5_0.
+Example add5_0_0 : combinational (adderGrowth (bv4_0, bv4_0)) = bv5_0.
 Proof. reflexivity. Qed.
 
 (* Check 1 + 2 = 3 *)
-Example add5_1_2 : combinational (addSim bv4_1 bv4_2) = bv5_3.
+Example add5_1_2 : combinational (adderGrowth (bv4_1, bv4_2)) = bv5_3.
 Proof. reflexivity. Qed.
 
 (* Check 15 + 1 = 16 *)
-Example add5_15_1 : combinational (addSim bv4_15 bv4_1) = bv5_16.
+Example add5_15_1 : combinational (adderGrowth (bv4_15, bv4_1)) = bv5_16.
 Proof. reflexivity. Qed.
 
 (* Check 15 + 15 = 30 *)
-Example add5_15_15 : combinational (addSim bv4_15 bv4_15) = bv5_30.
+Example add5_15_15 : combinational (adderGrowth (bv4_15, bv4_15)) = bv5_30.
 Proof. reflexivity. Qed.
 
 (******************************************************************************)
@@ -95,13 +102,8 @@ Definition adder4Interface
      (mkPort "sum" (BitVec Bit 5))
      [].
 
-Definition addNet {aSize bSize: nat}
-           (ab: Signal (BitVec Bit aSize) * Signal (BitVec Bit bSize)) :
-           state CavaState (Signal (BitVec Bit (1 + max aSize bSize))) :=
-  let (a, b) := ab in unsignedAdd a b.
-
 Definition adder4Netlist
-  := makeNetlist adder4Interface addNet.
+  := makeNetlist adder4Interface adderGrowth.
 
 Definition adder4_tb_inputs
   := [(bv4_0, bv4_0); (bv4_1, bv4_2); (bv4_15, bv4_1); (bv4_15, bv4_15)].
@@ -123,12 +125,12 @@ Definition adder8_3inputInterface
      (mkPort "sum" (BitVec Bit 10))
      [].
 
-Definition add3InputTuple {m bit vec} `{Cava m bit vec}
+Definition add3InputTuple {m bit} `{Cava m bit}
                           (aSize bSize cSize: nat)
-                          (abc: vec Bit aSize *
-                                vec Bit bSize *
-                                vec Bit cSize) :
-                          m (vec Bit (1 + max (1 + max aSize bSize) cSize)) :=
+                          (abc: Vector.t bit aSize *
+                                Vector.t bit bSize *
+                                Vector.t bit cSize) :
+                          m (Vector.t bit (1 + max (1 + max aSize bSize) cSize)) :=
   let '(a, b, c) := abc in adder_3input a b c.
 
 Definition adder8_3inputNetlist
