cava/monad-examples/AdderTree.v
@@ -38,19 +38,10 @@ Require Import Cava.Monad.UnsignedAdders.
 (* by using the tree combinator.                                              *)
 (******************************************************************************)
 
-(* List based adder tree *)
-Definition adderTree {m bit vec} `{Cava m bit vec} {sz: nat}
-                     (n: nat) (v: vec (BitVec Bit sz) (2^(n+1))) :
-                      m (vec Bit sz) :=
-  let vv : Vector.t (vec Bit sz) (2^(n+1)) := vecToVector2 Bit sz v in                
-  tree addNN defaultBitVec n vv.
-
-(* Vector based adder tree which currently does not work *)
-Definition adderTreeV  {m bit vec} `{Cava m bit vec} {sz: nat}
-                       (n: nat) (v: vec (BitVec Bit sz) (2^(n+1))) :
-                       m (vec Bit sz) :=
-  let vv : Vector.t (vec Bit sz) (2^(n+1)) := vecToVector2 Bit sz v in                
-  treeV n addNN vv.
+Definition adderTree {m bit} `{Cava m bit} {sz: nat}
+                     (n: nat) (v: Vector.t (Vector.t bit sz) (2^(n+1))) :
+                     m (Vector.t bit sz) :=              
+  tree n addNN v.
 
 (******************************************************************************)
 (* Some tests.                                                                *)
@@ -68,8 +59,8 @@ Local Open Scope string_scope.
 
 Local Open Scope nat_scope.
 
-Definition adderTree2 {m bit vec} `{Cava m bit vec} {sz}
-                      (v : vec (BitVec Bit sz) 2) : m (vec Bit sz)
+Definition adderTree2 {m bit} `{Cava m bit} {sz: nat}
+                      (v : Vector.t (Vector.t bit sz) 2) : m (Vector.t bit sz)
   := adderTree 0 v.
 
 Local Open Scope vector_scope.
@@ -82,12 +73,13 @@ Proof. reflexivity. Qed.
 
 (* An adder tree with 4 inputs. *)
 
-Definition adderTree4 {m bit} `{Cava m bit} {sz}
-                      (v : vec (BitVec Bit sz) 4) : m (vec Bit sz)
+Definition adderTree4 {m bit} `{Cava m bit} {sz: nat}
+                      (v : Vector.t (Vector.t bit sz) 4) : m (Vector.t bit sz)
   := adderTree 1 v.
 
 Definition v0_3 := [v0; v1; v2; v3].
 Definition sum_v0_3 : Bvector 8 := combinational (adderTree4 v0_3).
+Compute sum_v0_3.
 
 Example sum_v0_v1_v2_v3 : combinational (adderTree4 v0_3) = N2Bv_sized 8 30.
 Proof. reflexivity. Qed.
